

Linyi YE

A1. $U = \{(x, y) \mid x > 0, y > 0\}$

$$\phi: U \rightarrow \mathbb{R}^2 \text{ by } \phi(x, y) = (x^2 - y^2, xy).$$

Show that $\phi: U \rightarrow \mathbb{R}^2$ is a smooth change of variables.

Proof: ① obviously ϕ is a cont diff mapping.
To see this, the derivative matrix is given by.

$$\begin{pmatrix} 2x & y \\ -2y & x \end{pmatrix}$$

They are all continuous functions,
So ϕ is continuous differentiable.

$$\textcircled{2} D\phi = 2x^2 + 2y^2 > 0 \Rightarrow D\phi(x, y) \text{ is invertible}$$

$$\textcircled{3} \phi \text{ is } 1-1:$$

$$\text{let } s = x^2 - y^2, \quad t = xy.$$

We need to show that each (s, t)
gives a unique (x, y) .

This means solving for x, y in terms of s, t .
 of finding a unique sol.

$$\begin{cases} x^2 - y^2 = s & (1) \end{cases}$$

$$\begin{cases} xy = t & (2) \end{cases}$$

$$(1) \Rightarrow y^2 = x^2 - s$$

$$y = \sqrt{x^2 - s} \quad (y > 0)$$

$$(2) \Rightarrow xy = x \cdot \sqrt{x^2 - s} = t.$$

$$x^4 - x^2 \cdot s - t^2 = 0.$$

$$x^2 = \frac{s \pm \sqrt{s^2 + 4t^2}}{2}$$

$$\text{obviously } x^2 = \frac{s + \sqrt{s^2 + 4t^2}}{2} \quad (x^2 > 0)$$

$$\text{And } x = \sqrt{\frac{s + \sqrt{s^2 + 4t^2}}{2}} \quad (x > 0)$$

Thus x is unique.

$y = \frac{t}{x}$ is also unique.

So we get a unique (x, y)

This means $\phi: U \rightarrow \mathbb{R}^2$ is 1-1.

By the definition and ① ② ③, we prove that

$\phi: U \rightarrow \mathbb{R}^2$ is a smooth change of variables

A2. $D = \{(x, y) \mid x > 0, y > 0, 1 < x^2 - y^2 < 9, 2 < xy < 4\}$

P3

For a cont func $f: D \rightarrow \mathbb{R}$, Use hyperbolic coordinates from A1. to show

$$\int_D |x^2 + y^2| dx dy = 8.$$

Proof: From A1. We know.

$\phi: U \rightarrow \mathbb{R}$ is a smooth C-o-v.
 $\phi(x, y) = (x^2 - y^2, xy)$

Make $u = x^2 - y^2, t = xy$

$$x = \frac{t}{y} \Rightarrow u = \left(\frac{t}{y}\right)^2 - y^2 \Rightarrow y^2(u+1) = t^2. \quad y = \frac{t}{\sqrt{u+1}}$$

$$\Rightarrow x = \sqrt{u+1} \quad y = \frac{t}{\sqrt{u+1}}$$

By Th. 19.9 C-o-v th and Fubini's theorem

$$\int_{\phi(D)} f(x, y) dx dy = \int f(x(u, v), y(u, v)) \left| \frac{\partial(x, y)}{\partial(u, v)} \right| du dv$$

$$x^2 + y^2 = \sqrt{(x^2 - y^2)^2 + 4(xy)^2}$$

$$= \sqrt{u^2 + 4t^2}$$

$$\det \left| \frac{\partial(x,y)}{\partial(u,v)} \right| = \det \left| \frac{\partial(u,v)}{\partial(x,y)} \right| = \begin{pmatrix} 2x & -2y \\ y & x \end{pmatrix} = \frac{1}{2x^2 + 2y^2} = \frac{1}{2\sqrt{u^2 + 4v^2}}$$

The integral becomes -

$$\int_{\phi(D)} \frac{1}{2} du dv = \int_1^9 \int_2^4 \frac{1}{2} du dv = 8$$

A3. $f_n(x) = \sqrt{x^2 + \frac{1}{n}}$, $x \in (-1, 1)$.

§9.4 P254

#1

define $f(x) = |x|$

① Prove $\{f_n\} \xrightarrow{\text{uniform}} f$ on $(-1, 1)$.

② Check if f_n is C^1 , ($\lim f_n$ not diff at $x=0$)

③ Does this contradict Th. 9.33?

① uniform convergence.

Obviously $f_n(x) \xrightarrow{\text{pointwise}} f(x)$.

$$\lim_{n \rightarrow \infty} f_n(x) = \sqrt{x^2 + 0} = |x|.$$

$$\lim_{n \rightarrow \infty} [f_n(x) - f(x)] = \lim_{n \rightarrow \infty} \left(\sqrt{x^2 + \frac{1}{n}} - |x| \right)$$

$$= \lim_{n \rightarrow \infty} \frac{\frac{1}{n}}{\sqrt{x^2 + \frac{1}{n}} + \sqrt{x^2}}$$

$$\leq \lim_{n \rightarrow \infty} \frac{1}{n} / \sqrt{\frac{1}{n}}$$

$$= \lim_{n \rightarrow \infty} \frac{1}{\sqrt{n}} = 0.$$

Thus $\{f_n\} \xrightarrow{\text{uniform}} f$

$$\begin{aligned}
 \textcircled{2} \quad \frac{d f_n(x)}{dx} &= \left(\sqrt{x^2 + \frac{1}{n}} \right)' \\
 &= \frac{1}{2} \cdot \frac{2x}{\sqrt{x^2 + \frac{1}{n}}} \\
 &= \frac{x}{\sqrt{x^2 + \frac{1}{n}}}
 \end{aligned}$$

Obviously $f'_n(x)$ is a continuous func

$\Rightarrow f_n(x)$ is continuously differentiable

$\textcircled{3}$ No. Since, $f(x) = |x|$ is not differentiable at x .

$$\lim_{x \rightarrow 0} f(x) = \lim_{x \rightarrow 0} |x| = 0.$$

A4.

$$f_n(x) = nx e^{-nx^2}, \quad x \in [0, 1] \quad \text{p7}$$

§9.4 P254. ① Prove $\{f_n\} \xrightarrow{\text{Pointwise}} f = 0$.

#2.

② But $\left\{ \int_0^1 f_n \right\} \not\rightarrow 0$

③ Does this contradict Th. 9.32?

Proof: ① when $x=0$, $f_n(x)=0$.

when $x \neq 0$. Notice that $e^{nx^2} > \frac{n^2 x^4}{500}$.

Then $0 < nx e^{-nx^2} < \frac{500}{nx^3}$ $\lim_{n \rightarrow \infty} \frac{500}{nx^3} = 0$.

$\Rightarrow \lim_{n \rightarrow \infty} nx e^{-nx^2} = 0$ by sandwich

$\Rightarrow f_n(x) \rightarrow 0$ Pointwise.

② For $n \geq 1$, we have

$$\int_0^1 f_n(x) = -\frac{1}{2} e^{-nx^2} \Big|_0^1 = \frac{1}{2} (1 - e^{-n})$$

$\Rightarrow \lim_{n \rightarrow \infty} \int_0^1 f_n(x) = \frac{1}{2}$

③ $|f_n(x) - 0| = |nx e^{-nx^2}|$

$\stackrel{x = \frac{1}{\sqrt{n}}}{=} |\sqrt{n} \cdot e^{-1}|$

$\lim_{n \rightarrow \infty} |f_n(x)| = \infty \Rightarrow f_n(x) \not\Rightarrow 0$ ~~uniform~~

Hence, this does not contradict Th. 9.32

A5. Express $\sum_{n=1}^{\infty} x^n / n^2$ as an integral p8

$$\frac{x^n}{n^2} = \int_0^x \frac{t^{n-1}}{n} dt.$$

$$\begin{aligned} \text{So } \sum_{n=1}^{\infty} \frac{x^n}{n^2} &= \sum_{n=1}^{\infty} \int_0^x \frac{t^{n-1}}{n} dt \\ &= \int_0^x \left(\sum_{n=1}^{\infty} \frac{t^{n-1}}{n} \right) dt. \end{aligned}$$

$$\text{Since } \frac{x^n}{n} = \int_0^x t^{n-1} dt$$

$$\begin{aligned} \sum \frac{x^n}{n} &= \sum \int_0^x t^{n-1} dt \\ &= \int_0^x \sum t^{n-1} dt \\ &= \int_0^x \frac{1}{1-t} dt \\ &= -(\ln(1-t)) \end{aligned}$$

$$\Rightarrow \sum \frac{t^{n-1}}{n} = -\frac{1}{t} (\ln(1-t))$$

$$\Rightarrow \frac{x^n}{n^2} = \int_0^x -\frac{1}{t} (\ln(1-t)) dt$$